proof grinding

src/Dmajortodflatmajor.v
@@ -27,44 +27,9 @@ Variable prog: Dmajor.program.
 Let ge := Genv.globalenv prog.
 Hypothesis no_repet : list_norepet (prog_defs_names prog).
 
-(* Here we have a sufficient condition which we'll prove holds on all stack frames *)
+(* Well formedness of a stack frame in memory *)
 Definition stack_frame_wf (b : block) (stacksize : Z) (mi : meminj) (m : mem) : Prop :=
    Mem.range_perm m b 0 stacksize Cur Freeable /\ forall b' delta, mi b' <> Some (b,delta).
-
-Lemma free_stack_frame :
-  forall mi m m' b sz,
-    Mem.mem_inj mi m m' ->
-    stack_frame_wf b sz mi m' ->
-    exists m0,
-      Mem.free m' b 0 sz = Some m0 /\ Mem.mem_inj mi m m0.
-Proof.
-  intros.
-  unfold stack_frame_wf in *.
-  break_and.
-  app Mem.range_perm_free Mem.range_perm.
-  destruct H0.
-  app Mem.free_right_inj Mem.mem_inj.
-  intros.
-  specialize (H1 b' delta). congruence.
-Qed.
-
-Lemma free_stack_frame_inject :
-  forall mi m m' b sz,
-    Mem.inject mi m m' ->
-    stack_frame_wf b sz mi m' ->
-    exists m0,
-      Mem.free m' b 0 sz = Some m0 /\ Mem.inject mi m m0.
-Proof.
-  intros.
-  assert (Mem.mem_inj mi m m') by (inv H; eauto).
-  app free_stack_frame stack_frame_wf. 
-  app Mem.free_right_inject Mem.inject.
-  intros.
-  unfold stack_frame_wf in *. break_and.
-  specialize (H9 b1 delta). congruence.
-Qed.
-
-(* Here we have properties about the memory injection *)
 
 (* This says that our injection maps every old block to something new *)
 Definition total_inj (mi : meminj) (m : mem) : Prop :=
@@ -72,6 +37,12 @@ Definition total_inj (mi : meminj) (m : mem) : Prop :=
     Mem.load c m b ofs = Some v ->
     exists b',
       mi b = Some (b',0).
+
+(* Injection only deals with meaningful blocks *)
+Definition minimal_inj (mi : meminj) (m : mem) : Prop :=
+  forall b x,
+    mi b = Some x ->
+    Mem.valid_block m b.
 
 (* local variables follow our injection *)
 Definition env_inj (mi : meminj) (e e' : env) : Prop :=
@@ -88,11 +59,61 @@ Definition globals_inj_same (mi : meminj) : Prop :=
     mi b = Some (b,0).
 
 (* yet another useful property for a mapping function *)
-Definition meminj_injective ( mi : meminj) : Prop :=
+Definition meminj_injective (mi : meminj) : Prop :=
   forall b1 b2 b ofs1 ofs2,
     mi b1 = Some (b, ofs1) ->
     mi b2 = Some (b, ofs2) ->
     b1 = b2.
+
+(* nothing is moved around within blocks *)
+Definition same_offsets (mi : meminj) : Prop :=
+  forall b b' delta,
+    mi b = Some (b',delta) ->
+    delta = 0.
+
+(* conglomeration props *)
+Definition wf_inj (mi : meminj) : Prop :=
+  globals_inj_same mi /\
+  meminj_injective mi /\
+  same_offsets mi.
+
+Definition wf_mem (mi : meminj) (m : mem) : Prop :=
+  wf_inj mi /\ total_inj mi m /\ minimal_inj mi m.
+
+Lemma free_stack_frame_mem_inj :
+  forall mi m m' b sz,
+    Mem.mem_inj mi m m' ->
+    stack_frame_wf b sz mi m' ->
+    exists m0,
+      Mem.free m' b 0 sz = Some m0 /\ Mem.mem_inj mi m m0.
+Proof.
+  intros.
+  unfold stack_frame_wf in *.
+  break_and.
+  app Mem.range_perm_free Mem.range_perm.
+  destruct H0.
+  app Mem.free_right_inj Mem.mem_inj.
+  intros.
+  specialize (H1 b' delta). congruence.
+Qed.
+
+(* If we have a stack frame, we can free it and end up with still injecting memory *)
+Lemma free_stack_frame :
+  forall mi m m' b sz,
+    Mem.inject mi m m' ->
+    stack_frame_wf b sz mi m' ->
+    exists m0,
+      Mem.free m' b 0 sz = Some m0 /\ Mem.inject mi m m0.
+Proof.
+  intros.
+  assert (Mem.mem_inj mi m m') by (inv H; eauto).
+  app free_stack_frame_mem_inj stack_frame_wf. 
+  app Mem.free_right_inject Mem.inject.
+  intros.
+  unfold stack_frame_wf in *. break_and.
+  specialize (H9 b1 delta). congruence.
+Qed.
+
 
 Lemma globals_inj_find_symbol_same :
   forall i b mi,
@@ -119,13 +140,8 @@ Proof.
   repeat (econstructor; eauto).
 Qed.  
 
-Definition same_offsets (mi : meminj) : Prop :=
-  forall b b' delta,
-    mi b = Some (b',delta) ->
-    delta = 0.
-
 (* evaluating expressions translates *)
-Lemma eval_expr_mem_inj :
+Lemma eval_expr_mem_inj_parts :
   forall e m exp v,
     Dmajor.eval_expr ge e m exp v ->
     forall m' mi e' sp,
@@ -189,15 +205,31 @@ Proof.
     eauto.
 Qed.
 
-Lemma eval_exprlist_mem_inj :
+Lemma eval_expr_transf :
+  forall e m exp v,
+    Dmajor.eval_expr ge e m exp v ->
+    forall m' mi e' sp,
+      Mem.inject mi m m' ->
+      wf_mem mi m ->
+      env_inj mi e e' ->
+      exists v',
+        eval_expr ge e' m' sp exp v' /\ Val.inject mi v v'.
+Proof.
+  intros.
+  eapply eval_expr_mem_inj_parts; eauto.
+  inv H0. eauto.
+  inv H1. break_and. assumption.
+  inv H1. inv H3. assumption.
+  inv H1. inv H3. break_and. eauto.
+Qed.
+
+Lemma eval_exprlist_transf :
   forall l m e vl,
     Dmajor.eval_exprlist ge e m l vl ->
     forall m' mi e' sp,
-      Mem.mem_inj mi m m' ->
-      total_inj mi m ->
+      Mem.inject mi m m' ->
+      wf_mem mi m ->
       env_inj mi e e' ->
-      globals_inj_same mi ->
-      same_offsets mi ->
       exists vl',
         eval_exprlist ge e' m' sp l vl' /\ Val.inject_list mi vl vl'.
 Proof.
@@ -206,71 +238,10 @@ Proof.
   copy H1.
   eapply IHeval_exprlist in H1; eauto.
   break_exists; break_and.
-  eapply eval_expr_mem_inj in H; eauto.
+  eapply eval_expr_transf in H; eauto.
   break_exists; break_and.
   eexists; split; econstructor; eauto.
 Qed.  
-
-Inductive match_cont : Dmajor.cont -> Dflatmajor.cont -> Prop :=
-| match_stop :
-    match_cont Dmajor.Kstop Dflatmajor.Kstop
-| match_seq : forall s k k',
-    match_cont k k' ->
-    match_cont (Dmajor.Kseq s k) (Dflatmajor.Kseq s k')
-| match_block : forall k k',
-    match_cont k k' ->
-    match_cont (Dmajor.Kblock k) (Dflatmajor.Kblock k')
-| match_call : forall oid f e e' sp k k' mi,
-    match_cont k k' ->
-    env_inj mi e e' ->
-    match_cont (Dmajor.Kcall oid f e k) (Dflatmajor.Kcall oid f sp e' k').
-
-
-Inductive match_states : Dmajor.state -> Dflatmajor.state -> Prop :=
-| match_state : forall f s k k' b e e' m m' z mi,
-    Mem.inject mi m m' ->
-    stack_frame_wf b (fn_stackspace f) mi m' ->
-    match_cont k k' ->
-    total_inj mi m ->
-    env_inj mi e e' ->
-    globals_inj_same mi ->
-    same_offsets mi ->
-    meminj_injective mi ->
-    match_states
-      (Dmajor.State f s k e m)
-      (Dflatmajor.State f s k' (Vptr b Int.zero) e' m' z)
-| match_callstate : forall f args args' k k' m m' z mi,
-    Mem.inject mi m m' ->
-    match_cont k k' ->
-    total_inj mi m ->
-    globals_inj_same mi ->
-    same_offsets mi ->
-    Val.inject_list mi args args' ->
-    meminj_injective mi ->
-    match_states
-      (Dmajor.Callstate f args k m)
-      (Dflatmajor.Callstate f args' k' m' z)
-| match_returnstate : forall v v' k k' m m' z mi,
-    Mem.inject mi m m' ->
-    match_cont k k' ->
-    total_inj mi m ->
-    globals_inj_same mi ->
-    same_offsets mi ->
-    Val.inject mi v v' ->
-    meminj_injective mi ->
-    match_states
-      (Dmajor.Returnstate v k m)
-      (Dflatmajor.Returnstate v' k' m' z).
-
-Lemma is_call_cont_transf :
-  forall k k',
-    match_cont k k' ->
-    Dmajor.is_call_cont k ->
-    is_call_cont k'.
-Proof.
-  induction k; intros;
-    inv H; eauto.
-Qed.
 
 Lemma env_inj_set :
   forall mi e e',
@@ -289,33 +260,120 @@ Proof.
   eapply H; eauto.
 Qed.
 
-Lemma total_inj_store_mapped :
-  forall mi m,
-    total_inj mi m ->
-    forall c b ofs v m',
-      Mem.store c m b ofs v  = Some m' ->
-      exists b' delta,
-        mi b = Some (b',delta).
+
+Fixpoint highest_block (c : Dflatmajor.cont) : block :=
+  match c with
+  | Kstop => 1%positive
+  | Kseq _ k => highest_block k
+  | Kblock k => highest_block k
+  | Kcall _ _ sp _ k =>
+    let h := highest_block k in
+    match sp with
+    | Vptr b _ => Pos.max b h
+    | _ => h
+    end
+  end.
+
+(* Needs to have mem as an index or parameter *)
+(* since mem contains well formed stack frames *)
+(* and the cont is the runtime stack *)
+Inductive match_cont : Dmajor.cont -> Dflatmajor.cont -> meminj -> mem -> Prop :=
+| match_stop :
+    forall mi m,
+      match_cont Dmajor.Kstop Dflatmajor.Kstop mi m
+| match_seq : forall s k k' mi m,
+    match_cont k k' mi m ->
+    match_cont (Dmajor.Kseq s k) (Dflatmajor.Kseq s k') mi m
+| match_block : forall k k' mi m,
+    match_cont k k' mi m ->
+    match_cont (Dmajor.Kblock k) (Dflatmajor.Kblock k') mi m
+| match_call : forall oid f e e' b k k' mi m,
+    match_cont k k' mi m ->
+    env_inj mi e e' ->
+    stack_frame_wf b (fn_stackspace f) mi m ->
+    Plt (highest_block k') b ->
+    match_cont (Dmajor.Kcall oid f e k) (Dflatmajor.Kcall oid f (Vptr b Int.zero) e' k') mi m.
+
+
+Inductive match_states : Dmajor.state -> Dflatmajor.state -> Prop :=
+| match_state : forall f s k k' b e e' m m' z mi,
+    Mem.inject mi m m' ->
+    stack_frame_wf b (fn_stackspace f) mi m' ->
+    Plt (highest_block k') b ->
+    match_cont k k' mi m' ->
+    env_inj mi e e' ->
+    wf_mem mi m ->
+    match_states
+      (Dmajor.State f s k e m)
+      (Dflatmajor.State f s k' (Vptr b Int.zero) e' m' z)
+| match_callstate : forall f args args' k k' m m' z mi,
+    Mem.inject mi m m' ->
+    match_cont k k' mi m' ->
+    wf_mem mi m ->
+    Val.inject_list mi args args' ->
+    match_states
+      (Dmajor.Callstate f args k m)
+      (Dflatmajor.Callstate f args' k' m' z)
+| match_returnstate : forall v v' k k' m m' z mi,
+    Mem.inject mi m m' ->
+    match_cont k k' mi m' ->
+    wf_mem mi m ->
+    Val.inject mi v v' ->
+    match_states
+      (Dmajor.Returnstate v k m)
+      (Dflatmajor.Returnstate v' k' m' z).
+
+Lemma is_call_cont_transf :
+  forall k k' mi m,
+    match_cont k k' mi m ->
+    Dmajor.is_call_cont k ->
+    is_call_cont k'.
+Proof.
+  induction k; intros;
+    inv H; eauto.
+Qed.
+
+Lemma match_call_cont :
+  forall k k' mi m,
+    match_cont k k' mi m ->
+    match_cont (Dmajor.call_cont k) (call_cont k') mi m.
+Proof.
+  induction 1; intros; simpl; eauto; try solve [econstructor; eauto].
+Qed.
+
+Lemma Plt_pos_max_r :
+  forall x y z,
+    Plt (Pos.max x y) z ->
+    Plt y z.
 Proof.
   intros.
-  unfold total_inj in *.
-  app Mem.store_valid_access_3 Mem.store.
-  Check Mem.valid_access_load.
-  SearchAbout Mem.valid_access.
-  app Mem.valid_access_implies Mem.valid_access.
-  clear H2.
-  app Mem.valid_access_load Mem.valid_access.
-  edestruct H. eauto.
-  eexists. exists 0. app H (Mem.load c m b ofs).
-  econstructor; eauto.
+  destruct (Pos.max_spec x y);
+    break_and;
+  rewrite H1 in *; eauto.
+  unfold Plt in *.
+  eapply Pos.le_lt_trans; eauto.
+Qed.
+  
+Lemma Plt_pos_max_l :
+  forall x y z,
+    Plt (Pos.max x y) z ->
+    Plt x z.
+Proof.
+  intros.
+  destruct (Pos.max_spec x y);
+    break_and;
+  rewrite H1 in *; eauto.
+  unfold Plt in *.
+  eapply Pos.le_lt_trans; eauto.
+  eapply Pos.lt_eq_cases; eauto.
 Qed.
 
 Lemma stack_frame_wf_store :
   forall c m b ofs v m',
     Mem.store c m b ofs v = Some m' ->
-    forall b sz mi,
-      stack_frame_wf b sz mi m ->
-      stack_frame_wf b sz mi m'.
+    forall b' sz mi,
+      stack_frame_wf b' sz mi m ->
+      stack_frame_wf b' sz mi m'.
 Proof.
   intros. inv H0.
   econstructor; eauto.
@@ -323,6 +381,104 @@ Proof.
   intros.
   eapply Mem.perm_store_1; eauto.
 Qed.
+
+
+(* If we free a block higher than the largest stack block, stack is still well formed *)
+Lemma match_cont_free_stack_frame :
+  forall k k' m' x b lo hi mi,
+    match_cont k k' mi m' ->
+    Mem.free m' b lo hi = Some x ->
+    Plt (highest_block k') b ->
+    match_cont k k' mi x.
+Proof.
+  induction 1; intros; try solve [ econstructor; eauto].
+  simpl in H4.
+  assert (b0 <> b).
+  {
+    eapply Plt_pos_max_l in H4.
+    eapply Plt_ne in H4; congruence.
+  }
+  econstructor; eauto.
+  eapply IHmatch_cont; eauto.
+  eapply Plt_pos_max_r; eauto.
+  unfold stack_frame_wf in *.
+  break_and. split; eauto.
+  unfold Mem.range_perm in *. intros.
+  eapply H1 in H7.
+  eapply Mem.perm_free_1 in H3; eauto.
+Qed.  
+
+Lemma stack_frame_wf_alloc_mapped :
+  forall b z mi m,
+    stack_frame_wf b z mi m ->
+    z > 0 ->
+    forall lo hi m' b0 c v m'' bx,
+      Mem.alloc m lo hi = (m',b0) ->
+      Mem.store c m' b0 lo v  = Some m'' ->
+      stack_frame_wf b z (fun x => if peq x bx then Some (b0,0) else mi x) m''.
+Proof.
+  intros.
+  unfold stack_frame_wf in *.
+  break_and. split.
+  unfold Mem.range_perm in *.
+  intros.
+  eapply H in H4.
+  eapply Mem.perm_store_1; eauto.
+  eapply Mem.perm_alloc_1; eauto.
+  intros. break_match; eauto.
+
+  intro.
+  unfold Mem.range_perm in H.
+  specialize (H 0).
+  assert (Mem.valid_block m b) by
+      (eapply Mem.perm_valid_block; eapply H; omega).
+  unfold Mem.valid_block in *.
+  app Mem.alloc_result Mem.alloc.
+  subst b0.
+  match goal with
+  | [ H : Some _ = Some _ |- _ ] => inv H
+  end.
+  app Plt_ne Plt.
+  
+Qed.
+
+Lemma match_cont_store :
+  forall k k' m mi,
+    match_cont k k' mi m ->
+    forall c b ofs v m',
+      Mem.store c m b ofs v = Some m' ->
+      match_cont k k' mi m'.
+Proof.
+  induction 1; intros; try solve [econstructor; eauto].
+  econstructor; eauto.
+  eapply stack_frame_wf_store; eauto.
+Qed.
+
+Lemma match_cont_alloc_store :
+  forall k k' mi m,
+    match_cont k k' mi m ->
+    forall lo hi m' b c v m'' b0,
+      Mem.alloc m lo hi = (m',b) ->
+      Mem.store c m' b lo v = Some m'' ->
+      match_cont k k' (fun x => if peq x b0 then Some (b,0) else mi x) m''.
+Proof.
+  induction 1; intros; try solve [econstructor; eauto].
+  app stack_frame_wf_alloc_mapped stack_frame_wf.
+  econstructor; try eapply H1.
+  eauto.
+  unfold env_inj in *.
+  intros.
+  eapply H0 in H6.
+  break_exists. break_and.
+  eexists; split; eauto.
+  inv H7; econstructor; eauto.
+  admit. (* hmmm *)
+
+  eauto.
+
+  admit. (* need to thread it through *)
+Admitted.
+
 
 Lemma total_inj_store :
   forall c m b ofs v m',
@@ -339,77 +495,75 @@ Proof.
   clear H2. app H0 (Mem.load c0).
 Qed.
 
-Lemma no_overlap_store :
+Lemma minimal_inj_store :
   forall c m b ofs v m',
     Mem.store c m b ofs v = Some m' ->
     forall mi,
-      Mem.meminj_no_overlap mi m ->
-      Mem.meminj_no_overlap mi m'.
+      minimal_inj mi m ->
+      minimal_inj mi m'.
 Proof.
+  intros. unfold minimal_inj in *.
   intros.
-Admitted.
-
-
-Lemma symbols_inject_refl :
-  forall mi,
-    globals_inj_same mi ->
-    meminj_injective mi ->
-    symbols_inject mi ge ge.
-Proof.
-  intros.
-  unfold globals_inj_same in *.
-  unfold symbols_inject.
-  split. intros. reflexivity.
-  split. intros.
-  unfold Senv.find_symbol in *.
-  simpl in *.
-  app globals_inj_find_symbol_same Genv.find_symbol.
-  rewrite H1 in H2. inv H2. eauto.
-  split. intros. 
-  unfold Senv.find_symbol in *.
-  simpl in *.
-  app globals_inj_find_symbol_same Genv.find_symbol.
-  intros.
-  unfold Senv.block_is_volatile. simpl.
-  unfold Genv.block_is_volatile.
-  symmetry.
-  break_match.
-  erewrite H in H1; eauto.
-  inv H1. collapse_match. reflexivity.
-  
-  break_match; auto.
-  assert (mi b2 = Some (b2, 0)) by (eapply H; eauto).
-  unfold meminj_injective in *.
-  erewrite (H0 b1) in Heqo by eauto; congruence.
-  Unshelve.
-  repeat (econstructor; eauto).
-  repeat (econstructor; eauto).
-Qed.  
-
-Lemma match_call_cont :
-  forall k k',
-    match_cont k k' ->
-    match_cont (Dmajor.call_cont k) (call_cont k').
-Proof.
-  induction 1; intros; simpl; eauto; try solve [econstructor; eauto].
+  unfold Mem.valid_block in *.
+  erewrite Mem.nextblock_store; eauto.
 Qed.
 
-(* TODO: this lemma is duplicated from Emajortodmajor, make unified memory library *)
-Lemma alloc_store :
-  forall m lo hi m' b,
-    Mem.alloc m lo hi = (m',b) ->
-    forall v c,
-      hi - lo > size_chunk c ->
-      (align_chunk c | lo) ->
-      { m'' : mem | Mem.store c m' b lo v = Some m''}.
+
+Lemma wf_mem_store :
+  forall mi m,
+    wf_mem mi m ->
+    forall c b ofs v m',
+      Mem.store c m b ofs v = Some m' ->
+      wf_mem mi m'.
 Proof.
   intros.
-  app Mem.valid_access_alloc_same Mem.alloc; try omega.
+  unfold wf_mem in *.
+  break_and.
+  split. eauto.
+  split. eapply total_inj_store; eauto.
+  eapply minimal_inj_store; eauto.
+Qed.
+
+
+Lemma total_inj_store_mapped :
+  forall mi m,
+    total_inj mi m ->
+    forall c b ofs v m',
+      Mem.store c m b ofs v  = Some m' ->
+      exists b' delta,
+        mi b = Some (b',delta).
+Proof.
+  intros.
+  unfold total_inj in *.
+  app Mem.store_valid_access_3 Mem.store.
   app Mem.valid_access_implies Mem.valid_access.
-  2: instantiate (1 := Writable); econstructor; eauto.
-  eapply Mem.valid_access_store; eauto.
+  clear H2.
+  app Mem.valid_access_load Mem.valid_access.
+  edestruct H. eauto.
+  eexists. exists 0. app H (Mem.load c m b ofs).
+  econstructor; eauto.
 Qed.
 
+Lemma wf_mem_store_mapped :
+  forall mi m,
+    wf_mem mi m ->
+    forall c b ofs v m',
+      Mem.store c m b ofs v  = Some m' ->
+      exists b',
+        mi b = Some (b',0).
+Proof.
+  intros. unfold wf_mem in *.
+  break_and.
+  app total_inj_store_mapped total_inj.
+  exists x.
+  unfold wf_inj in *.
+  break_and.
+  unfold same_offsets in *.
+  rewrite H1. repeat f_equal.
+  eapply H5; eauto.
+Qed.
+
+(* TODO: Decompose this into smaller lemmas *)
 Lemma alloc_store_inject :
   forall m lo hi m' b c m'' v,
     Mem.alloc m lo hi = (m',b) ->
@@ -417,19 +571,13 @@ Lemma alloc_store_inject :
     forall mi m0 v',
       Mem.inject mi m m0 ->
       Val.inject mi v v' ->
-      total_inj mi m ->
-      globals_inj_same mi ->
-      same_offsets mi ->
-      meminj_injective mi ->
-      exists m0' m0'' b',
+      wf_mem mi m ->
+      exists m0' b' m0'',
       let mi' := (fun x => if peq x b then Some (b',0) else mi x) in
         Mem.alloc m0 lo hi = (m0',b') /\
         Mem.store c m0' b' lo v' = Some m0'' /\
         Mem.inject mi' m'' m0'' /\
-        total_inj mi' m'' /\
-        globals_inj_same mi' /\
-        same_offsets mi' /\
-        meminj_injective mi'.
+        wf_mem mi' m''.
 Proof.
 Admitted.
 
@@ -442,28 +590,30 @@ Proof.
   intros.
   
   inv H0; inv H;
-  try solve [inv H3;
+  try solve [invp match_cont;
              eexists; split; try eapply plus_one; econstructor; eauto];
-  do 3 (try match goal with
-        | [ H : Dmajor.eval_expr _ _ _ _ _ |- _ ] => eapply eval_expr_mem_inj in H; repeat break_exists; repeat break_and; try eassumption
-        | [ H : Dmajor.eval_exprlist _ _ _ _ _ |- _ ] => eapply eval_exprlist_mem_inj in H; repeat break_exists; repeat break_and; try eassumption
-            end);
-  match goal with
-  | [ H : Mem.inject _ _ _ |- Mem.mem_inj _ _ _ ] => solve [inversion H; eassumption]
-  | [ |- _ ] => idtac
-  end;
-  match goal with
-  | [ H : Mem.inject ?X ?Y ?Z |- _ ] =>
-    assert (Mem.mem_inj X Y Z) by (inversion H; auto)
-  end.
+  repeat match goal with
+        | [ H : Dmajor.eval_expr _ _ _ _ _ |- _ ] => eapply eval_expr_transf in H; repeat break_exists; repeat break_and; try eassumption
+        | [ H : Dmajor.eval_exprlist _ _ _ _ _ |- _ ] => eapply eval_exprlist_transf in H; repeat break_exists; repeat break_and; try eassumption
+         end.
 
-  * app free_stack_frame_inject stack_frame_wf; eauto.
+  (* Interesting case *)
+  (* Return from a function *)
+  (* Free a stack frame *)
+  * app free_stack_frame stack_frame_wf; eauto.
     eexists; split; try eapply plus_one; econstructor; eauto.
     eapply is_call_cont_transf; eauto.
+    eapply match_cont_free_stack_frame; eauto.
+      
   * eexists; split; try eapply plus_one; econstructor; eauto.
     eapply env_inj_set; eauto.
+
+  (* Interesting case *)
+  (* store to the heap *)
   * destruct vaddr; simpl in *; try congruence.
-    app total_inj_store_mapped total_inj.
+    instantiate (1 := (Vptr b Int.zero)) in H9.
+    instantiate (1 := (Vptr b Int.zero)) in H7.
+    app wf_mem_store_mapped wf_mem.
     app Mem.store_mapped_inject Mem.inject; try solve [invp Mem.inject; eauto].
     invp (Val.inject mi (Vptr b0 i)).
     eexists; split; try eapply plus_one; econstructor;
@@ -475,17 +625,16 @@ Proof.
     match goal with
     | [ H : Some _ = Some _ |- _ ] => inv H
     end.
-    match goal with
-    | [ H : same_offsets _, H2 : mi _ = Some _ |- _ ] =>
-      eapply H in H2; subst
-    end.
     rewrite Int.add_zero. rewrite Z.add_0_r in *. eauto.
-    eapply total_inj_store; eauto.
+    eapply match_cont_store; eauto.
+    eapply wf_mem_store; eauto.
+
   * eexists; split; try eapply plus_one; econstructor; eauto.
     destruct vfp; simpl in *; try congruence.
     unfold Genv.find_funct in *.
     break_match_hyp; try congruence. subst i.
     invp (Val.inject mi (Vptr b0 Int.zero)).
+    assert (globals_inj_same mi) by (unfold wf_mem in *; unfold wf_inj in *; break_and; eauto).
     match goal with
     | [ H : globals_inj_same _, H2 : mi _ = Some _ |- _ ] =>
       erewrite H in H2; eauto
@@ -509,10 +658,12 @@ Proof.
       end;
       eauto.
 
-    (* stack frame: not exactly sure where to go here *)
-    (* need to stick invariant in match_cont about all things being stack_frame_wf *)
-    admit.
+    eapply stack_frame_wf_alloc_mapped; eauto.
 
+    admit. (* need to thread it through *)
+    
+    eapply match_cont_alloc_store; eauto.
+    
     (* just env_inj proof here *)
     {
       unfold env_inj. intros.
@@ -531,54 +682,54 @@ Proof.
       unfold env_inj in *.
       app H5 (e ! id0).
       eexists; split; eauto.
-      inv H24; econstructor; eauto.
+      
+      inv H18; econstructor; eauto.
       find_rewrite.
       break_match; try congruence.
-      (* This case is weird, idk *)
-      admit.
+
+      subst.
+      match goal with
+      | [ H : wf_mem mi m, H2 : Mem.alloc m _ _ = _, H3 : mi _ = _ |- _ ] => clear -H H2 H3
+      end.
+      unfold wf_mem in *;
+        unfold wf_inj in *;
+        break_and.
+      unfold minimal_inj in *.
+
+      app Mem.alloc_result Mem.alloc.
+      (* haha backtracking match *)
+      match goal with
+      | [ H : _, H2: mi b0 = _ |- _ ] => eapply H in H2; clear H
+      end.
+
+      subst b0. unfold Mem.valid_block in *.
+      app Plt_ne Plt.
+      congruence.
     } 
 
-  * eexists; split; try eapply plus_one; econstructor; eauto.
+      * eexists; split; try eapply plus_one; econstructor; eauto.
     econstructor; eauto.
   * eexists; split; try eapply plus_one; econstructor; eauto.
     econstructor; eauto.
   * eexists; split; try eapply plus_one; econstructor; eauto.
-    inv H17; inv H10; econstructor; eauto.
-  * app free_stack_frame_inject stack_frame_wf.
+    invp switch_argument; invp Val.inject; econstructor; eauto.
+  * app free_stack_frame stack_frame_wf.
     eexists; split; try eapply plus_one; econstructor; eauto.
     eapply match_call_cont; eauto.
-  * app free_stack_frame_inject stack_frame_wf.
+    eapply match_cont_free_stack_frame; eauto.
+  * app free_stack_frame stack_frame_wf.
     eexists; split; try eapply plus_one; econstructor; eauto; try eapply match_call_cont; eauto.
+    eapply match_cont_free_stack_frame; eauto.
   * (* This is an interesting one *)
     (* we have to allocate memory *)
     (* but we don't have to stick it in the injection *)
-    
     admit.
   * inv H2.
     eexists; split; try eapply plus_one; try econstructor; eauto.
     (* match_cont needs Kcall to contain a Vptr for sp *)
     admit.
 
-    
-Unshelve.
-repeat (econstructor; eauto).
-repeat (econstructor; eauto).
-repeat (econstructor; eauto).
-repeat (econstructor; eauto).
-repeat (econstructor; eauto).
-repeat (econstructor; eauto).
-repeat (econstructor; eauto).
-repeat (econstructor; eauto).
-repeat (econstructor; eauto).
-repeat (econstructor; eauto).
-repeat (econstructor; eauto).
-repeat (econstructor; eauto).
-repeat (econstructor; eauto).
-repeat (econstructor; eauto).
-repeat (econstructor; eauto).
-repeat (econstructor; eauto).
-repeat (econstructor; eauto).
-    
+
 Admitted.
 
 End PRESERVATION.
